src/Parsers/ParserImplementation.v
@@ -62,6 +62,7 @@ Section implementation.
                         H' _ pf
                            (projT1 (parse_of_item__of__minimal_parse_of_item pit))
                            (projT1 (parse_of_production__of__minimal_parse_of_production pits))).
+          rewrite Min.min_r by assumption.
           apply H'; eauto.
           { erewrite <- parse_of_item_respectful_refl.
             eapply expand_forall_parse_of_item;
@@ -85,6 +86,7 @@ Section implementation.
           specialize (H' (length str) (reflexivity _)).
           pose proof (fun H => expand_minimal_parse_of_item (str' := take (length str) str) (or_introl (reflexivity _)) (reflexivity _) (or_introl (reflexivity _)) H pit) as pit'; clear pit.
           pose proof (fun H => expand_minimal_parse_of_production (str' := drop (length str) str) (or_introl (reflexivity _)) (reflexivity _) (or_introl (reflexivity _)) H pits) as pits'; clear pits.
+          rewrite Min.min_idempotent.
           refine ((fun ret => let pit'' := pit' (fst (snd ret)) in
                               let pits'' := pits' (snd (snd ret)) in
                               ((H' (projT1 (fst (fst ret) pit'')) (projT1 (snd (fst ret) pits'')) (projT2 (fst (fst ret) pit'')) (projT2 (snd (fst ret) pits'')), pit''), pits'')) _); repeat split.
